more properties of algorithmic typing

theories/AlgorithmicTyping.v
@@ -7,6 +7,67 @@ Section Definitions.
   instance *)
   Close Scope typing_scope.
 
+  Inductive ConvTypeAlg : context -> term -> term  -> Type :=
+    | typeConvRed {Γ A A' B B'} :
+      [A ⇒* A'] ->
+      [B ⇒* B'] ->
+      [Γ |- A' ≅h B'] ->
+      [Γ |- A ≅ B]
+  with ConvTypeRedAlg : context -> term -> term -> Type :=
+    | typePiCongAlg {Γ na na' A B A' B'} :
+      [ Γ |- A ≅ A'] ->
+      [ Γ ,, vass na A |- B ≅ B'] ->
+      [ Γ |- tProd na A B ≅h tProd na' A' B']
+    | typeUnivConvAlg {Γ} :
+      [Γ |- U ≅h U]
+    | typeNeuConvAlg {Γ M N} :
+      [ Γ |- M ~h N ▹ U ] -> 
+      [ Γ |- M ≅h N]
+  with ConvNeuAlg : context -> term -> term  -> term -> Type :=
+    | neuVarConvAlg {Γ n decl} :
+      in_ctx Γ n decl ->
+      [Γ |- tRel n ~ tRel n ▹ decl.(decl_type)]
+    | neuAppCongAlg {Γ m n t u na A B} :
+      [ Γ |- m ~h n ▹ tProd na A B ] ->
+      [ Γ |- t ≅ u : A ] ->
+      [ Γ |- tApp m t ~ tApp n u ▹ B[t..] ]
+  with ConvNeuRedAlg : context -> term -> term -> term -> Type :=
+    | neuConvRed {Γ m n A A'} :
+      [Γ |- m ~ n ▹ A] ->
+      [A ⇒* A'] ->
+      whnf A' ->
+      [Γ |- m ~h n ▹ A']
+  with ConvTermAlg : context -> term -> term -> term -> Type :=
+    | termConvRed {Γ t t' u u' A A'} :
+      [A ⇒* A'] ->
+      [t ⇒* t'] ->
+      [u ⇒* u' ] ->
+      [Γ |- t' ≅h u' : A'] ->
+      [Γ |- t ≅ u : A]
+  with ConvTermRedAlg : context -> term -> term -> term -> Type :=
+    | termPiCongAlg {Γ na na' A B A' B'} :
+      [ Γ |- A ≅ A' : U] ->
+      [ Γ ,, vass na A |- B ≅ B' : U] ->
+      [ Γ |- tProd na A B ≅h tProd na' A' B' : U]
+    | termFunConvAlg {Γ : context} {f g na A B} :
+      isFun f ->
+      isFun g ->
+      [ Γ,, vass na A |- eta_expand f ≅ eta_expand g : B] -> 
+      [ Γ |- f ≅h g : tProd na A B]
+    | termNeuConvAlg {Γ m n T N} :
+      [Γ |- m ~ n ▹ T] ->
+      whne N ->
+      [Γ |- m ≅h n : N]
+
+  where "[ Γ |- A ≅ B ]" := (ConvTypeAlg Γ A B)
+  and "[ Γ |- A ≅h B ]" := (ConvTypeRedAlg Γ A B)
+  and "[ Γ |- m ~ n ▹ T ]" := (ConvNeuAlg Γ T m n)
+  and "[ Γ |- m ~h n ▹ T ]" := (ConvNeuRedAlg Γ T m n)
+  and "[ Γ |- t ≅ u : T ]" := (ConvTermAlg Γ T t u)
+  and "[ Γ |- t ≅h u : T ]" := (ConvTermRedAlg Γ T t u)
+  and "[ t ⇒ t' ]" := (OneRedAlg t t')
+  and "[ t ⇒* t' ]" := (RedClosureAlg t t').
+
   Inductive WfTypeAlg : context -> term -> Type :=
     | wfTypeU Γ : [ Γ |- U ]
     | wfTypeProd {Γ na A B} :
@@ -42,69 +103,11 @@ Section Definitions.
       [ Γ |- t ▹ A ] -> 
       [ Γ |- A ≅ A'] -> 
       [ Γ |- t : A' ]
-  with ConvTypeAlg : context -> term -> term  -> Type :=
-    | typeConvRed {Γ A A' B B'} :
-      [A ⇒* A'] ->
-      [B ⇒* B'] ->
-      [Γ |- A' ≅h B'] ->
-      [Γ |- A ≅ B]
-  with ConvTypeRedAlg : context -> term -> term -> Type :=
-    | typePiCongAlg {Γ na na' A B A' B'} :
-      [ Γ |- A ≅ A'] ->
-      [ Γ ,, vass na A |- B ≅ B'] ->
-      [ Γ |- tProd na A B ≅h tProd na' A' B']
-    | typeUnivConvAlg {Γ} :
-      [Γ |- U ≅h U]
-    | typeNeuConvAlg {Γ M N} :
-      [ Γ |- M ~h N ▹ U ] -> 
-      [ Γ |- M ≅h N]
-  with ConvNeuAlg : context -> term -> term  -> term -> Type :=
-    | neuVarConvAlg {Γ n decl} :
-      in_ctx Γ n decl ->
-      [Γ |- tRel n ~ tRel n ▹ decl.(decl_type)]
-    | neuAppCongAlg {Γ m n t u na A B} :
-      [ Γ |- m ~h n ▹ tProd na A B ] ->
-      [ Γ |- t ≅ u : A ] ->
-      [ Γ |- tApp m t ~ tApp n u ▹ B[t..] ]
-  with ConvNeuRedAlg : context -> term -> term -> term -> Type :=
-    | neuConvRed {Γ m n A A'} :
-      [Γ |- m ~ n ▹ A] ->
-      [A ⇒* A'] ->
-      [Γ |- m ~h n ▹ A']
-  with ConvTermAlg : context -> term -> term -> term -> Type :=
-    | termConvRed {Γ t t' u u' A A'} :
-      [A ⇒* A'] ->
-      [t ⇒* t'] ->
-      [u ⇒* u' ] ->
-      [Γ |- t' ≅h u' : A'] ->
-      [Γ |- t ≅ u : A]
-  with ConvTermRedAlg : context -> term -> term -> term -> Type :=
-    | termPiCongAlg {Γ na na' A B A' B'} :
-      [ Γ |- A ≅ A' : U] ->
-      [ Γ ,, vass na A |- B ≅ B' : U] ->
-      [ Γ |- tProd na A B ≅h tProd na' A' B' : U]
-    | termFunConvAlg {Γ : context} {f g na A B} :
-      isFun f ->
-      isFun g ->
-      [ Γ,, vass na A |- eta_expand f ≅ eta_expand g : B] -> 
-      [ Γ |- f ≅h g : tProd na A B]
-    | termNeuConvAlg {Γ m n T N} :
-      [Γ |- m ~ n ▹ T] ->
-      whne N ->
-      [Γ |- m ≅h n : N]
 
   where "[ Γ |- A ]" := (WfTypeAlg Γ A)
   and "[ Γ |- t ▹ T ]" := (InferAlg Γ T t)
   and "[ Γ |- t ▹h T ]" := (InferRedAlg Γ T t)
-  and "[ Γ |- t : T ]" := (CheckAlg Γ T t)
-  and "[ Γ |- A ≅ B ]" := (ConvTypeAlg Γ A B)
-  and "[ Γ |- A ≅h B ]" := (ConvTypeRedAlg Γ A B)
-  and "[ Γ |- m ~ n ▹ T ]" := (ConvNeuAlg Γ T m n)
-  and "[ Γ |- m ~h n ▹ T ]" := (ConvNeuRedAlg Γ T m n)
-  and "[ Γ |- t ≅ u : T ]" := (ConvTermAlg Γ T t u)
-  and "[ Γ |- t ≅h u : T ]" := (ConvTermRedAlg Γ T t u)
-  and "[ t ⇒ t' ]" := (OneRedAlg t t')
-  and "[ t ⇒* t' ]" := (RedClosureAlg t t').
+  and "[ Γ |- t : T ]" := (CheckAlg Γ T t).
 
   (* Inductive WfContextAlgo : context -> Type :=
   | conNilAlg : [|- ε]
@@ -149,10 +152,6 @@ Section InductionPrinciples.
   Import AlgorithmicTypingData.
 
 Scheme 
-    Minimality for WfTypeAlg Sort Type with
-    Minimality for InferAlg Sort Type with
-    Minimality for InferRedAlg Sort Type with
-    Minimality for CheckAlg Sort Type with
     Minimality for ConvTypeAlg Sort Type with
     Minimality for ConvTypeRedAlg Sort Type with
     Minimality for ConvNeuAlg Sort Type with
@@ -160,19 +159,59 @@ Scheme
     Minimality for ConvTermAlg Sort Type with
     Minimality for ConvTermRedAlg Sort Type.
 
-Combined Scheme _WfAlgoInduction from
-    WfTypeAlg_rect_nodep,
-    InferAlg_rect_nodep,
-    InferRedAlg_rect_nodep,
-    CheckAlg_rect_nodep,
+Scheme
+    Minimality for WfTypeAlg Sort Type with
+    Minimality for InferAlg Sort Type with
+    Minimality for InferRedAlg Sort Type with
+    Minimality for CheckAlg Sort Type.
+
+Combined Scheme _AlgoConvInduction from
     ConvTypeAlg_rect_nodep,
     ConvTypeRedAlg_rect_nodep,
     ConvNeuAlg_rect_nodep,
     ConvNeuRedAlg_rect_nodep,
     ConvTermAlg_rect_nodep,
     ConvTermRedAlg_rect_nodep.
+
+Combined Scheme _AlgoTypingInduction from
+    WfTypeAlg_rect_nodep,
+    InferAlg_rect_nodep,
+    InferRedAlg_rect_nodep,
+    CheckAlg_rect_nodep.
+
+Definition AlgoConvInductionConcl
+  (PTyEq PTyRedEq : context -> term -> term -> Type)
+  (PNeEq PNeRedEq PTmEq PTmRedEq : context -> term -> term -> term -> Type) :=
+  (forall (Γ : context) (A B : term), [Γ |- A ≅ B] -> PTyEq Γ A B)
+  × (forall (Γ : context) (A B : term), [Γ |- A ≅h B] -> PTyRedEq Γ A B)
+  × (forall (Γ : context) (A m n : term), [Γ |- m ~ n ▹ A] -> PNeEq Γ A m n)
+  × (forall (Γ : context) (A m n : term), [Γ |- m ~h n ▹ A] -> PNeRedEq Γ A m n)
+  × (forall (Γ : context) (A t u : term), [Γ |- t ≅ u : A] -> PTmEq Γ A t u)
+  × (forall (Γ : context) (A t u : term), [Γ |- t ≅h u : A] -> PTmRedEq Γ A t u).
+
+Definition AlgoTypingInductionConcl
+  (PTy : context -> term -> Type)
+  (PInf PInfRed PCheck : context -> term -> term -> Type) :=
+  (forall (Γ : context) (A : term), [Γ |- A] -> PTy Γ A)
+  × (forall (Γ : context) (A t : term), [Γ |- t ▹ A] -> PInf Γ A t)
+  × (forall (Γ : context) (A t : term), InferRedAlg Γ A t -> PInfRed Γ A t)
+  × (forall (Γ : context) (A t : term), [Γ |- t : A] -> PCheck Γ A t).
+
+Definition AlgoConvInduction :=
+  ltac:(let ind := fresh "ind" in
+      pose (ind := _AlgoConvInduction);
+      fold_algo ;
+      let ind_ty := type of ind in
+      exact (ind : ind_ty)).
+
+Definition AlgoTypingInduction :=
+  ltac:(let ind := fresh "ind" in
+      pose (ind := _AlgoTypingInduction);
+      fold_algo ;
+      let ind_ty := type of ind in
+      exact (ind : ind_ty)).
     
-Definition WfAlgoInductionConcl
+(* Definition WfAlgoInductionConcl
   (PTy : context -> term -> Type)
   (PInf PInfRed PCheck PTyEq PTyRedEq : context -> term -> term -> Type)
   (PNeEq PNeRedEq PTmEq PTmRedEq : context -> term -> term -> term -> Type) :=
@@ -192,7 +231,7 @@ Definition WfAlgoInduction :=
       pose (ind := _WfAlgoInduction);
       fold_algo ;
       let ind_ty := type of ind in
-      exact (ind : ind_ty)).
+      exact (ind : ind_ty)). *)
 
 End InductionPrinciples.
 
@@ -219,11 +258,76 @@ Section TypingWk.
   Let PTmRedEq (Γ : context) (A t u : term) := forall Δ (ρ : Δ ≤ Γ), [|- Δ ] ->
       [Δ |- t⟨ρ⟩ ≅h u⟨ρ⟩ : A⟨ρ⟩].
 
-  Theorem typing_alg_wk :
-    WfAlgoInductionConcl PTy PInf PInfRed PCheck PTyEq PTyRedEq
+  Theorem algo_conv_wk :
+    AlgoConvInductionConcl PTyEq PTyRedEq
       PNeEq PNeRedEq PTmEq PTmRedEq.
   Proof.
-    apply WfAlgoInduction.
+    apply AlgoConvInduction.
+    - intros * ? ? ? IH.
+      econstructor.
+      1-2: eauto using credalg_wk.
+      now eapply IH.
+    - intros * ? IHA ? IHB ? *.
+      cbn.
+      econstructor.
+      1: now eapply IHA.
+      eapply (IHB _ (wk_up _ _ ρ)).
+      all: now econstructor.
+    - econstructor.
+    - intros * ? IHM.
+      econstructor.
+      now apply IHM.
+    - intros * ? ? ? ?.
+      eapply convne_meta_conv.
+      1: econstructor ; eauto using in_ctx_wk.
+      all: reflexivity.
+    - intros * ? IHm ? IHt ? ? ?.
+      cbn.
+      eapply convne_meta_conv.
+      1:{
+        econstructor.
+        2: now eapply IHt.
+        red in IHm ; cbn in IHm.
+        now eapply IHm.
+      }
+      1: asimpl.
+      all: reflexivity.
+    - intros * ? IHm ? ?.
+      econstructor.
+      + now apply IHm.
+      + eauto using credalg_wk.
+      + now eapply whnf_ren. 
+    - intros * ? ? ? ? IHt.
+      econstructor.
+      1-3: eauto using credalg_wk.
+      now eapply IHt.
+    - intros * ? IHA ? IHB ? ? ?.
+      cbn.
+      econstructor.
+      1: now eapply IHA.
+      eapply (IHB _ (wk_up _ _ ρ)).
+      all: now econstructor.
+    - intros ? f f' * ? ? ? IH ? ? ?.
+      cbn.
+      econstructor.
+      1-2: asimpl ; gen_typing.
+      specialize (IH _ (wk_up _ _ ρ)).
+      red in IH.
+      cbn in *.
+      asimpl.
+      repeat (erewrite compRenRen_term in IH ; [..|reflexivity]).
+      apply IH.
+      now econstructor.
+    - intros * ? IH ?.
+      econstructor.
+      2: cbn ; asimpl ; now gen_typing.
+      now eapply IH.
+  Qed.
+
+  Theorem algo_typing_wk :
+    AlgoTypingInductionConcl PTy PInf PInfRed PCheck.
+  Proof.
+    apply AlgoTypingInduction.
     - constructor.
     - intros Γ na A B HA IHA HB IHB Δ ρ HΔ.
       econstructor ; fold ren_term.
@@ -259,70 +363,10 @@ Section TypingWk.
       econstructor.
       + now eapply IHt.
       + eauto using credalg_wk.
-    - intros * ? IHt ? IHAA'.
+    - intros * ? IHt.
       econstructor.
       + now eapply IHt.
-      + now eapply IHAA'.
-    - intros * ? ? ? IH.
-      econstructor.
-      1-2: eauto using credalg_wk.
-      now eapply IH.
-    - intros * ? IHA ? IHB ? *.
-      cbn.
-      econstructor.
-      1: now eapply IHA.
-      eapply (IHB _ (wk_up _ _ ρ)).
-      all: now econstructor.
-    - econstructor.
-    - intros * ? IHM.
-      econstructor.
-      now apply IHM.
-    - intros * ? ? ? ?.
-      eapply convne_meta_conv.
-      1: econstructor ; eauto using in_ctx_wk.
-      all: reflexivity.
-    - intros * ? IHm ? IHt ? ? ?.
-      cbn.
-      eapply convne_meta_conv.
-      1:{
-        econstructor.
-        2: now eapply IHt.
-        red in IHm ; cbn in IHm.
-        now eapply IHm.
-      }
-      1: asimpl.
-      all: reflexivity.
-    - intros * ? IHm ?.
-      econstructor.
-      + now apply IHm.
-      + eauto using credalg_wk.
-    - intros * ? ? ? ? IHt.
-      econstructor.
-      1-3: eauto using credalg_wk.
-      now eapply IHt.
-    - intros * ? IHA ? IHB ? ? ?.
-      cbn.
-      econstructor.
-      1: now eapply IHA.
-      eapply (IHB _ (wk_up _ _ ρ)).
-      all: now econstructor.
-    - intros ? f f' * ? ? ? IH ? ? ?.
-      cbn.
-      econstructor.
-      1-2: asimpl ; gen_typing.
-      specialize (IH _ (wk_up _ _ ρ)).
-      red in IH.
-      cbn in *.
-      asimpl.
-      repeat (erewrite compRenRen_term in IH ; [..|reflexivity]).
-      apply IH.
-      now econstructor.
-    - intros * ? IH ?.
-      econstructor.
-      2: cbn ; asimpl ; now gen_typing.
-      now eapply IH.
+      + now eapply algo_conv_wk.
   Qed.
 
 End TypingWk.
-
-Import AlgorithmicTypingData.
